src/SDK/Serialize/Frames.dfy
@@ -1,0 +1,215 @@
+// Copyright Amazon.com Inc. or its affiliates. All Rights Reserved.
+// SPDX-License-Identifier: Apache-2.0
+
+include "../../../libraries/src/Collections/Sequences/Seq.dfy"
+include "../../Generated/AwsCryptographicMaterialProviders.dfy"
+include "../../AwsCryptographicMaterialProviders/Client.dfy"
+include "../../StandardLibrary/StandardLibrary.dfy"
+include "../../Util/UTF8.dfy"
+include "./SerializableTypes.dfy"
+include "SerializeFunctions.dfy"
+include "Header.dfy"
+include "EncryptionContext.dfy"
+include "EncryptedDataKeys.dfy"
+
+module Frames {
+  import Aws.Crypto
+  import Seq
+  import Header
+  import MaterialProviders.Client
+  import opened EncryptedDataKeys
+  import opened EncryptionContext2
+  import opened SerializableTypes
+  import opened StandardLibrary.UInt
+  import opened Wrappers
+  import opened UTF8
+  import opened SerializeFunctions
+
+  const START_SEQUENCE_NUMBER: uint32 := 1
+  const ENDFRAME_SEQUENCE_NUMBER: uint32 := 0xFFFF_FFFF
+                                        //  0x1_0000_0000
+  const NONFRAMED_SEQUENCE_NUMBER: uint32 := 1
+
+  type RegularFrameSequenceNumber = n: uint32
+  | n  < ENDFRAME_SEQUENCE_NUMBER
+  witness *
+
+  datatype Frame' = 
+  | RegularFrame(
+    header: Header.Header,
+    seqNum: RegularFrameSequenceNumber,
+    iv: seq<uint8>,
+    encContent: Uint8Seq32,
+    authTag: seq<uint8>)
+  | FinalFrame (
+    header: Header.Header,
+    finalSequenceNumber: uint32,
+    iv: seq<uint8>,
+    encContent: Uint8Seq32,
+    authTag: seq<uint8>)
+
+  type Frame = f: Frame'
+  |
+    && |f.iv| == f.header.suite.encrypt.ivLength as nat
+    && |f.authTag| == f.header.suite.encrypt.tagLength as nat
+  witness *
+
+  datatype NonFramed = NonFramed(
+    iv: seq<uint8>,
+    encContent: seq<uint8>,
+    authTag: seq<uint8>
+  )
+
+  function method WriteFrame(
+    frame: Frame
+  )
+    :(ret: seq<uint8>)
+    ensures 4  <= |ret|
+    ensures
+      ret[0..4] != UInt32ToSeq(ENDFRAME_SEQUENCE_NUMBER)
+    ==>
+      && frame.RegularFrame?
+      && ret == UInt32ToSeq(frame.seqNum)
+        + Write(frame.iv)
+        + Write(frame.encContent)
+        + Write(frame.authTag)
+    ensures
+      ret[0..4] == UInt32ToSeq(ENDFRAME_SEQUENCE_NUMBER)
+    ==>
+      && frame.FinalFrame?
+      && ret == UInt32ToSeq(ENDFRAME_SEQUENCE_NUMBER)
+        + UInt32ToSeq(frame.finalSequenceNumber)
+        + Write(frame.iv)
+        + UInt32ToSeq(|frame.encContent| as uint32)
+        + Write(frame.encContent)
+        + Write(frame.authTag)
+
+  {
+    match frame
+      case RegularFrame(_, seqNum, iv, encContent, authTag) =>
+        UInt32ToSeq(seqNum)
+        + Write(iv)
+        + Write(encContent)
+        + Write(authTag)
+      case FinalFrame(_, finalSequenceNumber, iv, encContent, authTag) =>
+        UInt32ToSeq(ENDFRAME_SEQUENCE_NUMBER)
+        + UInt32ToSeq(finalSequenceNumber)
+        + Write(iv)
+        + UInt32ToSeq(|encContent| as uint32)
+        + Write(encContent)
+        + Write(authTag)
+  }
+
+  function method ReadFrame(
+    bytes: ReadableBytes,
+    header: Header.Header
+  )
+    :(res: ReadCorrect<Frame>)
+    ensures CorrectlyRead(bytes, res, WriteFrame)
+  {
+    var sequenceNumber :- ReadUInt32(bytes);
+
+    if sequenceNumber.thing != ENDFRAME_SEQUENCE_NUMBER then
+      var iv :- Read(sequenceNumber.tail, header.suite.encrypt.ivLength as nat);
+      var encContent :- Read(iv.tail, header.body.frameLength as nat);
+      var authTag :- Read(encContent.tail, header.suite.encrypt.tagLength as nat);
+
+      var regularFrame: Frame := Frame'.RegularFrame(
+        header,
+        sequenceNumber.thing,
+        iv.thing,
+        encContent.thing,
+        authTag.thing
+      );
+
+      assert |WriteFrame(regularFrame)| == 4 + |iv.thing| + |encContent.thing| + |authTag.thing|;
+
+      assert WriteFrame(regularFrame)[bytes.start-bytes.start..sequenceNumber.tail.start-bytes.start] == sequenceNumber.tail.data[bytes.start..sequenceNumber.tail.start];
+      assert WriteFrame(regularFrame)[sequenceNumber.tail.start-bytes.start..iv.tail.start-bytes.start] == sequenceNumber.tail.data[sequenceNumber.tail.start..iv.tail.start];
+      assert WriteFrame(regularFrame)[iv.tail.start-bytes.start..encContent.tail.start-bytes.start] == sequenceNumber.tail.data[iv.tail.start..encContent.tail.start];
+      assert WriteFrame(regularFrame)[encContent.tail.start-bytes.start..authTag.tail.start-bytes.start] == sequenceNumber.tail.data[encContent.tail.start..authTag.tail.start];
+
+      assert CorrectlyRead(bytes, Success(Data(regularFrame, authTag.tail)), WriteFrame);
+      Success(Data(regularFrame, authTag.tail))
+    else
+      var finalSequenceNumber :- ReadUInt32(sequenceNumber.tail);
+      var iv :- Read(finalSequenceNumber.tail, header.suite.encrypt.ivLength as nat);
+      var contentLength :- ReadUInt32(iv.tail);
+      var encContent :- Read(contentLength.tail, contentLength.thing as nat);
+      var authTag :- Read(encContent.tail, header.suite.encrypt.tagLength as nat);
+
+      var finalFrame: Frame := Frame'.FinalFrame(
+        header,
+        finalSequenceNumber.thing,
+        iv.thing,
+        encContent.thing,
+        authTag.thing
+      );
+
+
+      assert |WriteFrame(finalFrame)| == 4 + 4 + |iv.thing| + 4 + |encContent.thing| + |authTag.thing|;
+
+      assert WriteFrame(finalFrame)[bytes.start-bytes.start..sequenceNumber.tail.start-bytes.start] == sequenceNumber.tail.data[bytes.start..sequenceNumber.tail.start];
+      assert WriteFrame(finalFrame)[sequenceNumber.tail.start-bytes.start..finalSequenceNumber.tail.start-bytes.start] == sequenceNumber.tail.data[sequenceNumber.tail.start..finalSequenceNumber.tail.start];
+      assert WriteFrame(finalFrame)[finalSequenceNumber.tail.start-bytes.start..iv.tail.start-bytes.start] == sequenceNumber.tail.data[finalSequenceNumber.tail.start..iv.tail.start];
+      assert WriteFrame(finalFrame)[iv.tail.start-bytes.start..contentLength.tail.start-bytes.start] == sequenceNumber.tail.data[iv.tail.start..contentLength.tail.start];
+      assert WriteFrame(finalFrame)[contentLength.tail.start-bytes.start..encContent.tail.start-bytes.start] == sequenceNumber.tail.data[contentLength.tail.start..encContent.tail.start];
+      assert WriteFrame(finalFrame)[encContent.tail.start-bytes.start..authTag.tail.start-bytes.start] == sequenceNumber.tail.data[encContent.tail.start..authTag.tail.start];
+
+      assert CorrectlyRead(bytes, Success(Data(finalFrame, authTag.tail)), WriteFrame);
+      Success(Data(finalFrame, authTag.tail))
+  }
+
+
+
+// function method ReadFinalFrame(
+//     bytes: ReadableBytes,
+//     header: Header.Header
+//   )
+//     :(res: ReadCorrect<Frame>)
+//     ensures CorrectlyRead(bytes, res, WriteFrame)
+//   {
+//     var sequenceNumber :- ReadUInt32(bytes);
+//     :- Need(sequenceNumber.thing != ENDFRAME_SEQUENCE_NUMBER, "asdf");
+      
+//     assert sequenceNumber.thing == ENDFRAME_SEQUENCE_NUMBER;
+//     var finalSequenceNumber :- ReadUInt32(sequenceNumber.tail);
+//     var iv :- Read(sequenceNumber.tail, header.suite.encrypt.ivLength as nat);
+//     var contentLength :- ReadUInt32(finalSequenceNumber.tail);
+//     var encContent :- Read(iv.tail, contentLength.thing as nat);
+//     var authTag :- Read(encContent.tail, header.suite.encrypt.tagLength as nat);
+
+//     var finalFrame: Frame := Frame'.FinalFrame(
+//       header,
+//       finalSequenceNumber.thing,
+//       iv.thing,
+//       encContent.thing,
+//       authTag.thing
+//     );
+
+//     Success(Data(finalFrame, authTag.tail))
+//   }
+
+
+
+
+
+
+
+  // The Encryption SDK no longer supports writing Non-Framed Data.
+  // That is why this is a function and not a function method.
+  // This is here to support correct reading of Non-Framed Data.
+  function WriteNonFramed(
+    nonFramed: NonFramed
+  )
+    :(ret: seq<uint8>)
+  {
+    Write(nonFramed.iv)
+    // Uint64 Length
+    + Write(nonFramed.encContent)
+    + Write(nonFramed.authTag)
+  }
+
+
+
+}
