src/SDK/Serialize/SerializeFunctions.dfy
@@ -85,7 +85,9 @@ module SerializeFunctions {
     length: nat
   ):
     (res: ReadBinaryCorrect<seq<uint8>>)
-    requires length > 0
+    // It may seem strange to alow reading 0 bytes
+    // however given compositional it is much more common than you might think.
+    // Optional elements in a data structure can be represented with a length of 0 bytes.
     ensures
       && |bytes.data| >= bytes.start + length
     ==>
